Tue Feb 28 11:10:49 PST 2017

## Homework Review
### p.65 #32
S1 = {7,8,9}

S2 = {2,3,6}

R1 = "<=" on S1

R2 = "1" on S2

R = lexicographic ordering on S1 x S2

Refer to figure `fig_228_1`
![Hasse Diagram](img/fig_228_1.png "fig_228_1")


### p.65 #42

S contains n elements

How many relations on S are anti-symmetric?

> recall a relation is a set of orderd pairs, 

> think of the set of all orderd pairs `S x S`

> think of building ar elation as picking a subset

> imagine s looke like this,

> S = {a1, a2, ..., an}

S1 : decide whether to include (a1,a1)

    N1 = 2

S2 : Decide whether to include (a2,a2)

    N2 = 2

...

Sn : Decide where to include (an,an)

    Nn = 2

more steps: each step has 3 possible outcomes

(a,b) (b,a)

n(n-1)

Altogether we get,

2^n * 3^(n(n-1)/2

anti-symetric relations

3^[] no of subsets of two distinct elments from S = 3^(n(n-1)/2


## Functions

**Definition:** A function f: `A->B` is a subset of `A x B` such that for each a∈A, there exists a unique b∈B with (a,b)∈ the subset of (AxB)

We usually denote b fy f(a).

Is R = {(a1,b1), (a2,b2), (a2,b3), (a3,b4), (a4,b5)}

a function of A = {a1,a2,a3,a4}

from B = {b1,b2,b3,b4,b5}

> What do you think?

> No.

> Why not?

> ... counting pairs. There should be 4 pairs, but we have 5.

What about R = {(a1,b1), (a2,b3), (a4,b5)} ?

> Should have 4 pairs? But we have 3. No.

How many functions are there from A to B?

S1: (a1, 5 choices)

S2: (a2, 5 choice)

S3: (a3, 5 choices)

S4: (a4, 5 choices)

by mult principle, there are 5^4 = 625 possible functions


R = { (a1,b1), (a2,b2), (a3,b3), (a4,b1) }

R is called a `consant function`.

For all a∈A, f(a)=b

Suppose A has m lemeents, and B has n elements.

then there are n^m functions, `f:A->B`

### Examples
Let S={a,b,c}, Let A=P(S), B={0,1,2,3,..,9} //i.e. decimal digits

Define f(a) = no. of elements in e

f(∅)=0

f({a})=1

...

f({a,b,c})=3


### Example
Suppose X is a set and A⊂X.

define f:X -> N by:

```
f_A(x) = { 1 if x∈A
           0 if x∉A }
```

f_A is called `characteristic function` of A.


### Example
Suppose A is any set.

Define f:A -> A by: 

f(a) = a for every a∈A.

f is called the `identity function`.

### Definition
A function `f:A->B` is called one-to-one (or 1-1) iff f(x)=f(y) => x=y for all x,y∈A

### Examples

Suppose A = {a,b,c,d}, B = {1,2,3,4,5,6}

f = {(a,1), (b,6), (c,4), (d,3)}

is a 1-1 function,

f' = {(a,2),(b,3),(c,2),(d,5)} is NOT 1-1.


### Example

Is f: Z -> Z, where f(n)=2n 1-1?

> Yes

**Proof:** (Direct Proof)

Assume: f(n) = f(m)

2n = 2m

=> n = m

&there4; f is 1-1.

### Example

Is f:N -> N defined by f(n) = n^2 1-1?

> Yes!

Suppose f(n) = f(m)

then n^2 = m^2

=> n^2 - m^2 = 0

=> (n-m)(n+m) = 0

=> Either n = m = 0, or n=m!=0

### Definition

A function f:A -> B is `onto` if, for every b&isin;B, here exists an element a&isin;A with f(a)=b

### Example:
Let A = {a,,c}, B={1,2,3}

f = {(a,1), (b,3), (c,2)} is onto

f' = {(a,3), (b,2),(c,3)} is not onto


### Terminology:

```
1-1 <--> "injection"
onto <--> "surjection"
1-1 and onto (both) <--> "bijection"
```

### Definition:
If f:A -> B is 1-1 and onto, we say that "A and B are in 1-1 correspondence". 


## take a break from Functions

### Example
What is the minimal elment in the set (0,1)?

### Well-Ordering Principle:
For every non-empty subset of the natural number shas a least element.

> not true for Real numbers, but is true for the natural numbers

### Principe of Mathematical Induction
Suppose S is a set of natural numbers that contains 1 and contains n+1 whenever it contains n. Then S = N.

**Proof by Contradiction**:

Suppose S is a set of natural numbers. 1∈S, and n+1∈S whenever n∈S.

Assume S' is non-empty.

Then S' must contain at least element k.

> Why? The WOP, "Well Ordering Principle"

Note that k!=1, since 1∈S. Since k is the least element in S',

it follows that k-1∈S. But k-1∈S => (k-1)+1 = k∈S.

Contradiction!

> What we're doing here is contradicting the WOP

### Example

Prove that for all natural numbers n, n^3- is divisible by 3.

**Proof by Induction:**

> There are two steps (two ingredients), in an induction proof

> reference the principle of matheaticla induction

> break down to 2 steps

(1) **Basis Step:** For n=1, 1^3-1=0, which is divisible by 3

(2) Assume that for some integer k, k^3-k is divisible by 3

Then (k+1)^3-(k+1)

= k^3 + 3k^2 + 3k + 1 - k - 1

= (k^3-k)+3(k^2+k)

= 3N+3(k^2+k)

= 3[N+k^2+k]


## Homework
* p.74 #1-5,7,8,9,11,

  45,47,49

  65,66

* p.84 #12-16,18
