Tue Apr  4 11:11:42 PDT 2017

# Review
## Example
How many Bridge hands contain a void suit?

Let A<sub>i</sub> = set of hands that are missing cards of i<sup>ith</sup> suit

We want | A<sub>1</sub> U A<sub>2</sub> U A<sub>3</sub> U A<sub>4</sub> |

= | A<sub>1</sub> | + | A<sub>2</sub> | + | A<sub>3</sub> | + | A<sub>4</sub> |

- |A<sub>1</sub> &cap; A<sub>2</sub> | - | A1 &cap; A3 | - | A1 &cap; A4 |

- | A2 &cap; A3 | - | A2 &cap; A4 | - | A3 &cap; A4 |

+ | A1 &cap; A2 &cap; A3 | + | A1 &cap; A2 &cap; A4 | + | A1 &cap; A3 &cap; A4 | + | A2 &cap; A3 &cap; A4 |

- | A1 &cap; A2 &cap; A3 &cap; A4 |

= 4 C(39,13) - C(4,2) C(26,13) + C(4,3) C(13,13) - 0

~= 3.24 * 10^10 

6.35 * 10^11 ~= 0.51 ~= 5%

## #7 from counting problem sheet

> was modeled off of 2 sticky problems from the book

> the book uses an `adding principle` that wasn't formally presented, but it's obvious that 2 unions of a set ....

```
 T       T       T
 O       T       T
 O       T       T
---     ---     ---

 T       T       T
 T       T       T
 0       0       T
---     ---     ---
```

```
choose kid to get 3 coins
|
v
3  * 7!/(3!3!1!)            T1 T2 ... T7
          ^
          |
          distribute toys


  3 * 7!/(3!2!2!)


= 7 6 5 4 3!
  ----------  (420)  
  2 3!               \
                       1050
     7 6 5 4 3!      /
  3 ----------- (630)
     3 2 2

```

> key is to break it into cases,

> think of adding principle as disjoint cases

## PHP #5

Consider the no's a1 , a2 , ... a36   1<= ai <= 50

where ai = no. of cases after i hours

these are distinct since there is at

least one case per hour

Condier the 36 no's

a1 + 21 , a2 + 21 , ... , a36 + 21

these are distinct.

Together, the two sets of numbers form a group of 72 integers between

1 and 71

By PHP, at least two are equal

i.e., for some i and j,

`aj = ai + 21`

# From last time

> inclusion/exclusion principle, talked a bit about onto, and partitions

## Reminder

No. of partitions of n elements into m disjoint subsets

= k=0, n &sum; (-1)^k (m-k)^n / (k!(m-k)! = {n,m}

= " n partition m"

> grows very quick, very very fast

## Another approach, is the Combinatorial Approach

*Note that:*

No. of partitions of { a1 , a2 , ... , an } into m subsets

= no. of partitions that leave an by itself

+ no. of partitions that have an included with other elements

<hr/>

> restriction: sets be non-empty

> ..."parallized disjoint?"

{ a , b , c , d }

{ a }  { b , c }  { d }

{ a , b } , { c } , { d }

{ a } , { b } , { c } , { d }

{ a , b , c } {d }

<hr/>

```
    d     d    d
    |     |    |
    v     v    v
   {a} , {b}, {c}
```

<hr/>

```
                                             Multiplication principle
                                            /
{ n , m } = { n-1 , m-1 } + { n-1, m } * m
```

> What does this remind you of?

> combinatorial?

> C(n,r) + C(n,r+1) = C(n+1,r+1)

> "Pascal's Identity"

> "Stirling's Triangle"

# Induction is important! 1 prob midterm, 1 on final
## #10, Guess a general rule?
( 1 - 1/4 )( 1 - 1/9 )( 1 - 1/16) ... ( 1 - 1/n^2 )

> suspicious about the form of this

> going to re-write it

```
   4 - 1     9 - 1    16 - 1           (n-1)^2 - 1      n^2 - 1
= ------- * ------- * ------  * ... * -------------  * ---------
     4         9        16              (n-1)^2            n^2
```

> there should be a lot of cancelation

```
   (2-1)(2+1)    (3-1)(3+1)   (4-1)(4+1)           (n-1)^2-1          n^2-1
= ----------- * ----------- * ----------  * ... * -------------  * ---------
     2^2            3^2           4^2              (n-1)^2            n^2

```

= n+1/(2n)

> write it out on a table

| n | - |
|---|---|
|2|3/4|
|3|2/3|
|4|5/8|

> it works! now we gotta do the proof by induction, should be the easy part

*Proof By Induction:*

(1) *Basis Step*: For n=2, (1 - 1/2^2) = 3/4 = 2+1 / (2\*2) &check;

(2) *Induction Hypothesis:*

assume that for some integer k>=2,

(1-1/4)(1-1/9) ...(1-1/k^2) = (k+1)/2k

then `(1-1/4)(1-1/9)...(1-1/k^2)`(1-1/(k+1)^2

= k+1/2k * (1-1/(k+1)^2)

= k+1/(2k)[(k+1)^2 - 1/(k+1)^2] = k(k+2)/(2k(k+1))

= k+2/[2(k+1)] = (k+1)+1/[2(k+1)] &check;


## More Induction, #5
For all positive integers n, 21 divides 4<sup>n+1</sup> + 5<sup>2n-1</sup>

> result is given, suppose to be true, don't need to do anything

> all we have to do is generate the proof, by induction

**Proof By Induction:**
(1) Basis Step: For n=1, 4<sup>n+1</sup> + 5<sup>2n-1</sup> = 4<sup>2</sup> + 5<sup>1</sup> = 16 + 5 = 21 &check;

(2) **Induction Hypothesis:** Assume there is a positive integer k with 4<sup>k+1</sup> + 5<sup>2k-1</sup> = 21 * L

> that's the induction hypothesis, now we gotta test the case k+1?

then 4<sup>(k+1)+1</sup> + 5<sup>2(k+1)-1</sup>

= 4 * 4<sup>k+1</sup> + 5<sup>(2k-1)</sup> * 25

= 25 [ 4<sup>k+1</sup> + 5<sup>2k-1</sup>] - 21 * 4<sup>k+1</sup>

= 21 [ 25 L - 4<sup>k+1</sup> ] which is an integer multiple of 21

> need to some way make use of the induction hypothesis

> only way to exploit it was...


## Example, Combinatorial Proof?
C(k,m) C(t,m) = C(t,m) C(t-m,t-k)

> put it into context

Consider a contest with t entrants.

there are C(t,k) ways to pick k semi-finalists

there are then C(k,m) ways to pick m finalists

altogether, there are C(k,m) C(t,k) wys to pick k semi-finalists and m finalists.

> this is the multiplication way?

<hr/>

> can do this backwards, by picking the finalists first

we can count this as follows:

S1: pick m finalists : N1 = C(t,m)

S2: pick the other k-m semi-finalists : N2 = C(t-m, k-m) = C(t-m,t-k)

(t-m) - (k-m) = t - k



