Thu Mar  9 11:13:20 PST 2017

## Questions from Homework
### From the Handout:
1\*2\*3 + 2\*3\*4 + 3\*4\*5 + ... + n(n+1)(n+2) = n(n+1)(n+2)(n+3)/4 for pos integers n.

**Proof By Induction**

(1) Basis Step: For n=1, 1\*2\*3 = 1\*(1+1)(1+2)(1+3)/4 = 1\*2\*3

(2) Induction Hypothesis: Suppose 

1\*2\*3 + 2\*3\*4 + ... + k(k+1)(k+2) = k(k+1)(k+2)(k+3)/4 for k = some pos integer

then 1\*2\*3 + 2\*3\*4 + ... + k(k+1)(k+2) + (k+1)(k+2)(k+3)

= k(k+1)(k+2)(k+3)/4 + (k+1)(k+2)(k+3)

= k(k+1)(k+2)(k+3)/4 + 4(k+1)(k+2)(k+4)/4 

= (k+1)(k+2)(k+3)(k+4)/4 = (k+1)((k+1)+1)([k+1]+2)([k+1]+3)/4

### From the handout:
For all pos integers n>=2, x^n - 1 is divisible by (x-1)

**Proof By Induction**:

**(1) Basis Step:** check for n=2, x^2 - 1 is (x+1)(x-1)

&there4; (x^2 - 1) is divisible by (x-1) 

**(2) Induction Hypothesis:**

Assume that or some positive integer k>=2,

x^k - 1 is divisible by (x-1).

this means that there exists a polynomial P(x) such that

x^k - 1 = P(x)(x-1)

> some polynomial times (x-1)

then x^(k+1) - 1

> need to look at the next case, the k+1 case

= x^(k+1) - x^k + x^k - 1

= x^k(x-1) + P(x)(x-1)

= (x-1) * [ x^k + P(x) ].

since P(x) is a polynomial, 

x^k + P(x) is a polynomial

&there4; x^k - 1 = polynomial * (x-1)

=> x^<sup>(k+1)</sup> is divisible by (x-1)



## Jumping ahead to Chapter 8, and look at section 2.6

**Recall:** The number of permutations of `n` objects taken `r` at-a-time

is: <sub>n</sub>P<sub>r</sub> = n!/(n-r)!

### For example:

Find the number of ways to line up 6 of 9 people in a row of chairs.

> We could use the multiplication principle, and have 6 steps,

> saying it's 9 * 8 * 7 * 6 * 5 * 4

or use the shortcut,

<sub>9</sub>P<sub>6</sub> = 9!/3! = 9\*8\*7\*6\*5\*4\*3!/3! = ...

Let's recount the number of was to permute `r` out of `n` objects:

S<sub>1</sub>: Select `r` objects to be arranged

  N<sub>1</sub> = ?

S<sub>2</sub>: Arrange the r selected objects:
  
  N<sub>2</sub> = r!

So, N<sub>1</sub>\*r! = <sub>n</sub>P<sub>r</sub>

N<sub>1</sub> = <sub>n</sub>P<sub>r</sub>/r!

### Definition

An unordered selection of `r` out of `n` objects is called a `combination`

of `n` objects taken `r` at-a-time.

By the multiplication principle, the number of combinations of `n` objects

taken `r` at-a-time is:

C(n,r) = <sub>n</sub>C<sub>r</sub> = <sub>n</sub>P<sub>r</sub>/r! = n!/[r!(n-r)!]

### Example

A committee has 8 members.

How many 3-member subcommittes are possible?

Number of 3-member subcommittees is: <sub>8</sub>C<sub>3</sub> = 8!/(3!5!) = 56

### Note

<sub>n</sub>C<sub>r</sub> = the number of `r`-element subsets a set with `n` elements has.

So,

 nC0 + nC1 + nC2 + ... + nCn-1 + nCn = 2<sup>n</sup>

**Formal Proof**

that nCr = n!/(r!(n-r)!)

**Proof:**

**(1) Basis Step:** For n=1,

the no. of o-element subsets

is 1, and 1!/[o!(1-o)!] = 1/(1\*1) = 1

the number of 1-element subsets 

is 1, and 1!/[1!(1-1)!] = 1/(1\*1) = 1

**(2) Induction Hypothesis**:

Assume that for some positive itneger k,

kCr = k!/[r!(k-r)!] for every integer r, 0<=r<=k.

Then, for k+1, the number of r element subsets

from a set with k+1 elements is equal to:

`number of subsets of size r not containing elt.x` + `no. of subsets of size r containing elt.x` = k!/[r!(k-r)!] + k!/[ (r-1)![k-(r-1)]! ]

= k!(k-r+1)/[r!(k-r)!(k-r+1) + k!\*r/[(r-1)!(k-r+1)!]\*r

= (k+1)\*k!/[r!(k-r+1)!]

Finally, for r=k+1,

there is just 1 subset of size k+1

and (k+1)!/(k+1)! = 1/(1\*1) = 1

> Which was more illuminating? Using multiplication principle, or through mathematical induction?

> Mathematical induction doesn't really show insight to anything. It's just

> to say, we have a hypothesis, and it's correct

> Multiplication principle had more insight?

### Prove: <sub>n</sub>C<sub>r</sub> = <sub>n</sub>C<sub>n-r</sub> (Symmetry Property)

**Combinatorial Proof:**

Note that <sub>n</sub>C<sub>r</sub> is the number of ways

to select `r out of `n` objects.

Every such selection determines a set

of `n-r` objects left un-selected. (and vice-versa)

&there4; the number of `r` objects subsets = number of `n-r` object subsets.

> BTW, this is usually called the `Symmetry Property`


<sub>n</sub>C<sub>r</sub> = n!/(r!(n-r)!)

= n!/( (n-r)![n-(n-r)]! )

= <sub>n</sub>C<sub>n-r</sub> 

### Prove: <sub>n</sub>C<sub>r</sub> + <sub>n</sub>C<sub>r+1</sub> = <sub>n+1</sub>C<sub>r+1</sub> 

```
n+1 objects

           x

n others
```

`number of r+1 elt subsets` = <sub>n+1</sub>C<sub>r+1</sub> 

= `no. of r+1 elt. subsets containing` + `no. of r+1 elt subset not containing x`

= <sub>n</sub>C<sub>r</sub> + <sub>n</sub>C<sub>r+1</sub> 

### ...

(A+B)<sup>2</sup> = (A+B)(A+B)

= AA + AB + BA + BB

= A<sup>2</sup>+2AB+B<sup>2</sup>

(A+B)<sup>3</sup> = (A+B)(A+B)(A+B)

= (A+B)(AA+AB+BA+BB)

= AAA + AAB + ABA + ABBB + BAA + BAB + BBA + BBB

= A<sup>3</sup> +3A<sup>2</sup> B + 3AB<sup>2</sup>  + B<sup>3</sup> 

(A+B)<sup>4</sup> = C(4,4)A<sup>4</sup> + C(r,3)A<sup>3</sup>B + C(4,2)A<sup>2</sup>B<sup>2</sup> + C(4,1)AB<sup>3</sup> + C(4,0)B<sup>4</sup> 

> <sub>n</sub>C<sub>r</sub> = (<sup>n</sup><sub>r</sub>) = "n choose r" = binomial coefficients

### Definition
For n = positive integers,

(A+B)<sup>n</sup> = &sum;<sup>n</sup><sub>k=0</sub>(<sup>n</sup><sub>k</sub>)A<sup>n-k</sup>B<sup>k</sup>

(Binomial Theorem)

(n 0) + (n 1) + (n 2) + ... + (n n) = 2<sup>n</sup>

= k=0 &sum; n (n k) 1^(n-k) * 1^k

= (1+1)^n = 2^n


nCr = nCr+1 = n+1Cr+1

Pascal's Identity (aka, hockey stick identity, or the xmas stocking identity)

```
1
1 1
1 2 1
1 3 3 1 = 8 
1 4 6 4 1 = 16
1 5 10 10 5 1 = 32
1 6 15 20 15 6 1
```


## Homework
p91, #1-12, #13-23(odd), #24,25,27

ch8 p405, #1-5, 7,9-25(odd)

